ExpReal revisited

test/testMasterLR.dfy
@@ -1,3 +1,4 @@
+include "../theory/math/ExpNat.dfy"
 include "../theory/math/ExpReal.dfy"
 include "../theory/math/LemBoundsNat.dfy"
 include "../theory/math/LemFunction.dfy"
@@ -7,6 +8,7 @@ include "../theory/math/TypeR0.dfy"
 include "../theory/ComplexityR0.dfy"
 include "../theory/MasterLR.dfy"
 
+import Nat = ExpNat
 import opened ExpReal
 import opened LemBoundsNat
 import opened LemFunction
@@ -144,9 +146,9 @@ lemma lem_T3def(n:nat)
 }
 
 // Exact closed form:
-//   T2(n) = 1/4*(2*n - (-1)^n - (-1)^(2 n) - 2)
+//   T3(n) = 1/4*(2*n - (-1)^n - (-1)^(2 n) - 2)
 // Asymptotic closed form:
-//   T2(n) in O(n)
+//   T3(n) in O(n)
 lemma test_masterMethodForT3lifted() 
   ensures liftToR0(T3) in O(n => exp(n as R0, 1.0))
 {
@@ -177,3 +179,74 @@ lemma test_masterMethodForT3lifted()
   } 
   thm_masterMethodLR(a, b, c, s, T3', w, k); 
 } 
+
+//**************************************************************************//
+
+// Recurrence 4:
+//   T4(n) = / 0                   , n <= 2
+//           \ 2*T4(n-2) + 3*n^2   , n > 2
+opaque ghost function T4(n:nat) : nat
+  decreases n
+{
+  if n <= 2
+  then 0   
+  else 2*T4(n-2) + 3*Nat.exp(n,2)
+}
+
+lemma lem_T4def(n:nat)
+  ensures n <= 2 ==> T4(n) == 0
+  ensures n > 2  ==> T4(n) == 2*T4(n-2) + 3*Nat.exp(n,2) 
+{
+  reveal T4();
+}
+
+// Exact closed form:
+//   T4(n) = ... hard
+// Asymptotic closed form by MT:
+//   T4(n) ∈ O(n^2*2^(n/2))
+// Thiger bound:
+//   T4(n) ∈ Θ(2^(n/2)) 
+lemma test_masterMethodForT6() 
+  ensures liftToR0(T4) in O(n => ((n*n) as R0)*exp(2.0, n as R0 / 2.0))
+{ 
+  var a:nat       := 2;
+  var b:nat       := 2;
+  var c:R0        := 0.0;
+  var s:nat       := 2;
+  var k:R0        := 2.0;
+  var T4':nat->R0 := liftToR0(T4);
+  var w:nat->R0   := liftToR0(n => 3*Nat.exp(n,2));
+
+  forall n:nat 
+    ensures T4'(n) == TbodyLR(a, b, c, s, T4', w, n)
+  {
+    reveal TbodyLR;
+    lem_T4def(n);
+  } 
+  assert w in O(n => exp(n as R0, k)) by {
+    // we show that c=3 and n0=1
+    forall n:nat | 0 <= 1 <= n
+      ensures w(n) <= 3.0*exp(n as R0, k)
+    {
+      reveal Nat.exp();
+      assert exp(n as R0, 2.0) == (n*n) as R0 by { lem_exp_Pow2(n as R0); } 
+      assert w(n) <= 3.0*exp(n as R0, k);  
+    }
+    assert bigOfrom(3.0, 1, w, n => exp(n as R0, k));
+  } 
+  thm_masterMethodLR(a, b, c, s, T4', w, k);
+  lem_simplifyPowrTwo();
+}
+
+lemma lem_simplifyPowrTwo() 
+  requires liftToR0(T4) in O(n => exp(n as R0, 2.0)*exp(2.0, n as R0 / 2.0))
+  ensures  liftToR0(T4) in O(n => ((n*n) as R0)*exp(2.0, n as R0 / 2.0))
+{  
+  assert forall n:nat :: exp(n as R0, 2.0) == (n*n) as R0 
+    by { lem_exp_Pow2Auto(); }
+  lem_fun_Ext((n:nat) => exp(n as R0, 2.0)*exp(2.0, n as R0 / 2.0), 
+              (n:nat) => ((n*n) as R0)*exp(2.0, n as R0 / 2.0)) by {
+    assert forall n:nat :: ((n:nat) => exp(n as R0, 2.0)*exp(2.0, n as R0 / 2.0))(n)
+                        == ((n:nat) => ((n*n) as R0)*exp(2.0, n as R0 / 2.0))(n);
+  }            
+}
