theory/ComplexityNat.dfy
@@ -12,6 +12,7 @@ include "./ComplexityR0.dfy"
 ******************************************************************************/
 
 module ComplexityNat {
+  
   import opened ExpNat
   import opened Factorial  
   import opened FloorCeil
