theory/math/LogReal.dfy
@@ -21,7 +21,7 @@ module LogReal {
     requires b > 1.0
     ensures  log(b, 1.0) == 0.0
 
-  // b > 1 /\ x >= 1 ==> log_b(x) >= 0
+  // b > 1 ∧ x >= 1 ==> log_b(x) >= 0
   lemma {:axiom} lem_log_NonNegative(b:real, x:real)
     requires b > 1.0 && x >= 1.0 
     ensures  log(b, x) >= 0.0 
